IndSim.v
@@ -21,49 +21,40 @@ Context (freeze : SimOpt.freeze_opt) (lock : SimOpt.lock_opt) (delay : SimOpt.de
 Notation Observable := lts.(Observable).
 Notation St := lts.(St).
 Notation trans := lts.(trans).
-Notation epsilon := lts.(epsilon).
+(*Notation epsilon := lts.(epsilon).*)
 Notation Robs := lts.(Robs).
 Notation ub_state := lts.(ub_state).
 Notation label := (@label Observable).
 
-  (* TODO try to just use TauAnswer with Rind as Rdiv *)
-  Variant TauIndAnswer (R Rind : relation St) s' t : Prop :=
-  | taui_exact t' (TR : trans tau t t') (SIM : R s' t')
-  | taui_freeze (_ : freeze = SimOpt.freeze) (SIM : R s' t)
-  | taui_div (_ : freeze = SimOpt.freeze_div) (SIM : Rind s' t)
-  | taui_delay t' (_ : delay = SimOpt.delay) (TR : (trans tau)^+ t t') (SIM : R s' t')
-  .
-  Hint Constructors TauIndAnswer : optsim.
+Definition simIndF R Rind s t :=
+  (forall o s', trans (obs o) s s' ->
+    ObsAnswer delay R s' t o
+  ) /\
+  (forall s', trans tau s s' ->
+    TauAnswer freeze delay R Rind s' t
+  ) /\
+  (lock = SimOpt.nolock \/ (is_stuck s -> can_be_stuck delay t)).
 
-  Definition simIndF R Rind s t :=
-    (forall o s', trans (obs o) s s' ->
-      ObsAnswer delay R s' t o
-    ) /\
-    (forall s', trans tau s s' ->
-      TauAnswer freeze delay R Rind s' t
-    ) /\
-    (lock = SimOpt.nolock \/ (is_stuck s -> can_be_stuck delay t)).
+Section NoElim.
+#[local] Unset Elimination Schemes.
+Inductive simInd R s t : Prop :=
+| simI :
+  simIndF R (simInd R) s t -> simInd R s t.
+End NoElim.
 
-  Section NoElim.
-  #[local] Unset Elimination Schemes.
-  Inductive simInd R s t : Prop :=
-  | simI :
-    simIndF R (simInd R) s t -> simInd R s t.
-  End NoElim.
-
-  Definition simInd_ind :
-    forall R P : St -> St -> Prop,
-         (forall s t : St,
-           (simIndF R (fun s t => simInd R s t /\ P s t) s t) -> 
-          P s t) -> forall t t0 : St, simInd R t t0 -> P t t0.
-  Proof.
-    intros until 1. fix F 3. intros. apply H. destruct H0. repeat split; intros.
-    - apply H0 in H1 as [].
-      eleft; eauto.
-      eright; eauto.
-    - apply H0 in H1 as []; esim.
-    - apply H0.
-  Qed.
+Definition simInd_ind :
+  forall R P : St -> St -> Prop,
+       (forall s t : St,
+         (simIndF R (fun s t => simInd R s t /\ P s t) s t) ->
+        P s t) -> forall t t0 : St, simInd R t t0 -> P t t0.
+Proof.
+  intros until 1. fix F 3. intros. apply H. destruct H0. repeat split; intros.
+  - apply H0 in H1 as [].
+    eleft; eauto.
+    eright; eauto.
+  - apply H0 in H1 as []; esim.
+  - apply H0.
+Qed.
 
 Lemma simInd_mon : forall R R', R <= R' -> simInd R <= simInd R'.
 Proof.
